



PARUL UNIVERSITY
Faculty of Engineering & Technology
Department of Applied Sciences and Humanities
1ST SEMESTER B.Tech PROGRAMME (CSE, IT)
CALCULUS(03019101BS01)
ACADEMIC YEAR – 2025-26

Tutorial 2A: Multivariate Calculus

Q. 1 Evaluate the following limits, if exists:

a) $\lim_{(x,y) \rightarrow (0,0)} \frac{x^3 - y^3}{x^2 + y^2}$ b) $\lim_{(x,y) \rightarrow (0,1)} \frac{x^2 + y^2 + 1}{3 + x^2 + 3y^2}$ c) $\lim_{(x,y) \rightarrow (0,0)} \frac{x+y}{x^2 + y^2}$ d) $\lim_{(x,y) \rightarrow (0,0)} \frac{x^3 + 2y^3}{x^2 + 4y^2}$

Q. 2 Check whether the given function is continuous or not, if yes then find point of continuity.

a) $f(x, y) = \begin{cases} \frac{x^2 y^2}{2x^2 + y^2}, & (x, y) \neq (0, 0) \\ 0 & (x, y) = (0, 0) \end{cases}$ b) $f(x, y) = \begin{cases} \frac{xy}{x^2 + xy + y^2}, & (x, y) \neq (0, 0) \\ 0 & (x, y) = (0, 0) \end{cases}$

Q. 3 If $u = x^3 y + e^{xy^2}$, show that $\frac{\partial^2 u}{\partial x \partial y} = \frac{\partial^2 u}{\partial y \partial x}$.

Q. 4 If $u = (x^2 + y^2 + z^2)^{-\frac{1}{2}}$, prove that $\frac{\partial^2 u}{\partial x^2} + \frac{\partial^2 u}{\partial y^2} + \frac{\partial^2 u}{\partial z^2} = 0$.

Q. 5 If $z(x + y) = x^2 + y^2$, show that $\left(\frac{\partial z}{\partial x} - \frac{\partial z}{\partial y}\right)^2 = 4\left(1 - \frac{\partial z}{\partial x} - \frac{\partial z}{\partial y}\right)$.

Q. 6 If $u = \operatorname{cosec}^{-1}\left(\sqrt{\frac{\frac{1}{x^2} + \frac{1}{y^2}}{\frac{1}{x^3} + \frac{1}{y^3}}}\right)$, show that $x^2 \frac{\partial^2 u}{\partial x^2} + 2xy \frac{\partial^2 u}{\partial x \partial y} + y^2 \frac{\partial^2 u}{\partial y^2} = \frac{1}{12} \tan u \left[\frac{13}{12} + \frac{1}{12} \tan^2 u\right]$.

Q. 7 Use the Chain Rule to find $\frac{dw}{dt}$ for $w = x e^{y/z}$, $x = t^2$, $y = 1 - t$, $z = 1 + 2t$.

Q. 8 If $y \log(\cos x) = x \log(\sin y)$, find $\frac{dy}{dx}$.

Q. 9 If $z = f(x, y)$ where $x = e^u + e^{-v}$, $y = e^{-u} - e^v$, prove that $\frac{\partial z}{\partial u} - \frac{\partial z}{\partial v} = x \frac{\partial z}{\partial x} - y \frac{\partial z}{\partial y}$.

Q. 10 If $u = f\left(\frac{y-x}{xy}, \frac{z-x}{xz}\right)$, then prove that $x^2 \frac{\partial u}{\partial x} + y^2 \frac{\partial u}{\partial y} + z^2 \frac{\partial u}{\partial z} = 0$.